src/cddl/pulse/CDDL.Pulse.AST.Parse.ElemType.fst
@@ -13,28 +13,6 @@ module S = Pulse.Lib.Slice
 module SZ = FStar.SizeT
 
 [@@AST.sem_attr]
-let impl_copyful_elem_type
-  (#ty: Type0)
-  (vmatch: (perm -> ty -> cbor -> slprop))
-  (cbor_get_major_type: get_major_type_t vmatch)
-  (cbor_destr_int64: read_uint64_t vmatch)
-  (cbor_get_string: get_string_t vmatch)
-  (cbor_destr_simple: read_simple_value_t vmatch)
-  (freeable: bool)
-  (l: AST.elem_typ { AST.wf_elem_typ l })
-: Tot (impl_copyful_parse vmatch (AST.spec_of_elem_typ l ()).parser (rel_elem_type_sem vmatch (AST.target_type_of_elem_typ l) freeable true))
-= match l returns (impl_copyful_parse vmatch (AST.spec_of_elem_typ l ()).parser (rel_elem_type_sem vmatch (AST.target_type_of_elem_typ l) freeable true)) with
-  | AST.ELiteral l -> impl_copyful_unit vmatch _
-  | AST.EBool -> impl_copyful_bool cbor_destr_simple
-  | AST.ESimple -> impl_copyful_simple cbor_destr_simple
-  | AST.EByteString -> impl_copyful_bytes cbor_get_string freeable
-  | AST.ETextString -> impl_copyful_text cbor_get_string freeable
-  | AST.EUInt -> impl_copyful_uint cbor_destr_int64
-  | AST.ENInt -> impl_copyful_nint cbor_destr_int64
-  | AST.EAlwaysFalse -> impl_copyful_always_false vmatch _
-  | AST.EAny -> impl_copyful_either_skip _ _
-
-[@@AST.sem_attr]
 let impl_zero_copy_elem_type
   (#ty: Type0)
   (vmatch: (perm -> ty -> cbor -> slprop))
@@ -42,10 +20,9 @@ let impl_zero_copy_elem_type
   (cbor_destr_int64: read_uint64_t vmatch)
   (cbor_get_string: get_string_t vmatch)
   (cbor_destr_simple: read_simple_value_t vmatch)
-  (skippable: bool)
   (l: AST.elem_typ { AST.wf_elem_typ l })
-: Tot (impl_zero_copy_parse vmatch (AST.spec_of_elem_typ l ()).parser (rel_elem_type_sem vmatch (AST.target_type_of_elem_typ l) false skippable))
-= match l returns (impl_zero_copy_parse vmatch (AST.spec_of_elem_typ l ()).parser (rel_elem_type_sem vmatch (AST.target_type_of_elem_typ l) false skippable)) with
+: Tot (impl_zero_copy_parse vmatch (AST.spec_of_elem_typ l ()).parser (rel_elem_type_sem vmatch (AST.target_type_of_elem_typ l)))
+= match l returns (impl_zero_copy_parse vmatch (AST.spec_of_elem_typ l ()).parser (rel_elem_type_sem vmatch (AST.target_type_of_elem_typ l))) with
   | AST.ELiteral l -> impl_zero_copy_unit vmatch _
   | AST.EBool -> impl_copyful_pure_as_zero_copy (impl_copyful_bool cbor_destr_simple)
   | AST.ESimple -> impl_copyful_pure_as_zero_copy (impl_copyful_simple cbor_destr_simple)
@@ -54,4 +31,4 @@ let impl_zero_copy_elem_type
   | AST.EUInt -> impl_copyful_pure_as_zero_copy (impl_copyful_uint cbor_destr_int64)
   | AST.ENInt -> impl_copyful_pure_as_zero_copy (impl_copyful_nint cbor_destr_int64)
   | AST.EAlwaysFalse -> impl_zero_copy_always_false vmatch _
-  | AST.EAny -> impl_zero_copy_either_skip _ (impl_zero_copy_any vmatch)
+  | AST.EAny -> (impl_zero_copy_any vmatch)
